src/tls/PNE.fst
@@ -51,27 +51,27 @@ assume val aes: lbytes 16 -> lbytes 16 -> lbytes 16
 
 #reset-options "--z3rlimit 50"
 
-let encrypt #i #u st n c =
+let encrypt #i #u st #l n c =
   let s = sample_cipher c in
   let t = PNE_state?.tbl st in
   let k = PNE_state?.key st in
-  let l = U32.uint_to_t pnlen in
+  let l' = U32.uint_to_t l in   
   if safePNE i then
-    (let ne = CoreCrypto.random pnlen in
+    (let ne = CoreCrypto.random l in
     t := Seq.snoc (!t) (Entry s ne n);
     ne)
   else
-    (let mask = Bytes.slice (aes k s) 0ul l in
-    let ne = Bytes.xor l (repr i u n) mask in
+    (let mask = Bytes.slice (aes k s) 0ul l' in 
+    let ne = Bytes.xor l' (repr i u l n) mask in
     t := Seq.snoc (!t) (Entry s ne n);
     ne)
   
 
-let decrypt #i #u st ne c =
+let decrypt #i #u st #l ne c =
   let s = sample_cipher c in
   let t = PNE_state?.tbl st in
   let k = PNE_state?.key st in
-  let l = U32.uint_to_t pnlen in
+  let l' = U32.uint_to_t l in
   if safePNE i then
     (match Seq.find_l (sample_filter i u s) !t with
           | None -> None
@@ -79,6 +79,6 @@ let decrypt #i #u st ne c =
             if ne = ne' then Some n
             else None)
   else
-    (let mask = Bytes.slice (aes k s) 0ul l in
-    let n = Bytes.xor l ne mask in
-    Some (abs i u n))
+    (let mask = Bytes.slice (aes k s) 0ul l' in
+    let n = Bytes.xor l' ne mask in
+    Some (abs i u l n))
