src/tls/QUICStream.fsti
@@ -3,6 +3,7 @@ module HS = FStar.HyperStack
 
 module I = Crypto.Indexing
 module U32 = FStar.UInt32
+module U64 = FStar.UInt64
 module U128 = FStar.UInt128
 module Plain = Crypto.Plain
 
@@ -21,6 +22,8 @@ type safeid = i:I.id{Flag.safeId i}
 
 let safeId (i:I.id) = AEAD.safeId i
 
+let safePNE (j:I.id) = PNE.safePNE j
+
 val plain: i:I.id -> l:plainLen -> t:Type0{hasEq t}
 
 val plain_as_bytes : i:I.id -> l:plainLen -> p:plain i l -> GTot (lbytes l)
@@ -29,32 +32,52 @@ val mk_plain: i:I.id -> l:plainLen -> b:lbytes l -> p:plain i l{~(AEAD.safeId i)
 
 val plain_repr : i:I.id{~(AEAD.safeId i)} -> l:plainLen -> p:plain i l -> b:lbytes l{b == plain_as_bytes i l p}
 
-type cipher (i:I.id) (l:plainLen) = lbytes l
+type cipher (i:I.id) (l:plainLen) = lbytes (l + v AEAD.taglen)
 
 let max_ctr = pow2 32 - 1
 
+type npn_length =
+  | OneByte
+  | TwoBytes
+  | FourBytes
+
 let pnlen = PNE.pnlen
 
-val pn: j:I.id -> t:Type0{hasEq t}
+let pnlen_of_npn_length (l:npn_length) : pnlen =
+  match l with
+    | OneByte -> 1
+    | TwoBytes -> 2
+    | FourBytes -> 4
 
-val pn_as_bytes : j:I.id -> n:pn j -> GTot (lbytes pnlen)
+val npn: j:I.id -> l:pnlen -> t:Type0{hasEq t}
 
-val mk_pn: j:I.id -> b:lbytes pnlen -> n:pn j{~(PNE.safePNE j) ==> pn_as_bytes j n == b}
+val npn_as_bytes : j:I.id -> l:pnlen -> n:npn j l -> GTot (lbytes l)
 
-val pn_repr : j:I.id{~(PNE.safePNE j)} -> n:pn j -> b:lbytes pnlen{b == pn_as_bytes j n}
+val mk_npn: j:I.id -> l:pnlen -> b:lbytes l -> n:npn j l{~(PNE.safePNE j) ==> npn_as_bytes j l n == b}
 
-type epn = PNE.epn
+val npn_repr : j:I.id{~(PNE.safePNE j)} -> l:pnlen -> n:npn j l -> b:lbytes l{b == npn_as_bytes j l n}
 
-let pn_as_nat (j:I.id) (n:pn j) : GTot (n:nat{n < pow2 32}) =
-  int_of_bytes (pn_as_bytes j n)
+let epn = PNE.epn
+
+let npn_as_nat (j:I.id) (l:pnlen) (n:npn j l) : GTot (m:nat{m < pow2 (Mul.op_Star 8 l)}) =
+  int_of_bytes (npn_as_bytes j l n)
+
+type rpn = n:U64.t{U64.v n <= pow2 62 - 1}
+
+let rpn_of_u32 (j:U32.t) : rpn =
+  let jj:nat = U32.v j in
+  U64.uint_to_t jj
+
+val npn_of_rpn : (j:I.id) -> (r:rpn) -> (l:pnlen) -> (n:npn j l)
 
 type stream_entry (i:I.id) (j:I.id) =
   | Entry:
-    pn: pn j ->
+    nl:pnlen ->
+    pn: rpn ->
     ad:AEAD.adata ->
     #l:plainLen ->
     p:plain i l ->
-    ne: epn ->
+    ne: epn nl ->
     c:cipher i l ->
     stream_entry i j
 
@@ -65,20 +88,20 @@ val stream_reader: #i:I.id -> #j:I.id -> w:stream_writer i j -> Type0
 val invariant: #i:I.id -> #j:I.id -> w:stream_writer i j -> mem -> Type0
 val rinvariant: #i:I.id -> #j:I.id -> #w:stream_writer i j -> r:stream_reader w -> h:mem -> Type0
 
-val wctrT: #i:I.id -> #j:I.id -> w:stream_writer i j -> mem -> GTot nat
+val wctrT: #i:I.id -> #j:I.id -> w:stream_writer i j -> mem -> GTot (n:nat{n<=max_ctr})
 val wctr: #i:I.id -> #j:I.id -> w:stream_writer i j -> ST UInt32.t
   (requires fun h0 -> True)
   (ensures fun h0 c h1 -> h0 == h1 /\ UInt32.v c = wctrT w h1)
 
-val read_pnT: #i:I.id -> #j:I.id -> #w: stream_writer i j -> r:stream_reader w -> h:mem ->
-  GTot (s:Seq.seq (pn j){rinvariant r h /\ safeId i ==> (forall (k:pn j). Seq.mem k s ==> pn_as_nat j k <= wctrT w h)})
+val pnlogT: #i:I.id -> #j:I.id -> #w: stream_writer i j -> r:stream_reader w -> h:mem ->
+  GTot (s:Seq.seq rpn{rinvariant r h /\ safeId i ==> (forall (k:pn j). Seq.mem k s ==> pn_as_nat j k <= wctrT w h)})
   
-val read_pn: #i:I.id -> #j:I.id -> #w: stream_writer i j -> r:stream_reader w -> ST (Seq.seq (pn j))
+val pnlog: #i:I.id -> #j:I.id -> #w: stream_writer i j -> r:stream_reader w -> ST (Seq.seq (pn j))
   (requires fun h0 -> True)
-  (ensures fun h0 s h1 -> h0 == h1 /\ s == read_pnT r h0)
+  (ensures fun h0 s h1 -> h0 == h1 /\ s == pnlogT r h0)
 
-val wlog: #i:safeid -> #j:I.id -> w:stream_writer i j -> h:mem -> GTot (s:Seq.seq (stream_entry i j)
-  {invariant w h ==> wctrT w h == Seq.length s})
+val wlog: #i:safeid -> #j:I.id -> w:stream_writer i j -> h:mem{invariant w h} -> GTot (s:Seq.seq (stream_entry i j)
+  {wctrT w h == Seq.length s})
 
 let pn_filter (i:I.id) (j:I.id) (ns:Seq.seq (pn j)) (e:stream_entry i j) : bool =
   let n = Entry?.pn e in
@@ -95,7 +118,7 @@ let log_filter (#i:safeid) (#j:I.id) (w:stream_writer i j) (h:mem{invariant w h}
 
 val rlog: #i:safeid -> #j:I.id -> #w:stream_writer i j -> r:stream_reader w -> h:mem{invariant w h /\ rinvariant r h} ->
   GTot (s:Seq.seq (stream_entry i j)
-    {s == log_filter w h (read_pnT r h)})
+    {s == log_filter w h (pnlogT r h)})
 
 
 
@@ -142,16 +165,18 @@ val rframe_invariant: #i:I.id -> #j:I.id -> #w:stream_writer i j -> r:stream_rea
     ~(Set.mem ri (shared_footprint w)))
   (ensures rinvariant r h1)
 
-val frame_log: #i:I.id -> #j:I.id -> w:stream_writer i j -> l:Seq.seq (stream_entry i j) ->
+
+val frame_log: #i:safeid -> #j:I.id -> w:stream_writer i j -> l:Seq.seq (stream_entry i j) ->
   h0:mem -> ri:rid -> h1:mem ->
   Lemma
   (requires
     Flag.safeId i /\
-//    invariant w h0 ->
+    invariant w h0 ->
     wlog w h0 == l /\
     modifies_one ri h0 h1 /\
-    ~(Set.mem ri (footprint w)))
-  (ensures wlog w h1 == l)
+    ~(Set.mem ri (footprint w)) /\
+    ~(Set.mem ri (shared_footprint w)))
+  (ensures invariant w h1 ==> wlog w h1 == l)
 
 
 val create: i:I.id -> j:I.id -> u:info i j ->
@@ -188,7 +213,7 @@ val createReader: parent:rgn -> #i:I.id -> #j:I.id -> w:stream_writer i j ->
     modifies_none h0 h1 /\
     Flag.safeId i ==>
       (rlog r h1 == Seq.empty /\
-      read_pnT r h1 == Seq.empty)
+      pnlogT r h1 == Seq.empty)
   )
 
 
@@ -201,15 +226,16 @@ val encrypt
   (#j:I.id)
   (w:stream_writer i j)
   (ad:AEAD.adata)
+  (nl:pnlen)
   (l:plainLen)
   (p:plain i l):
-  ST (epn*(cipher i l))
+  ST ((epn nl) * (cipher i l))
   (requires fun h0 -> wincrementable w h0 /\ invariant w h0)
   (ensures fun h0 (ne,c) h1 ->
     invariant w h1 /\
     wctrT w h1 == wctrT w h0 + 1 /\ 
     (Flag.safeId i ==> (
-      exists (n:pn j). (wlog w h1 == Seq.snoc (wlog w h0) (Entry n ad p ne c) /\ wctrT w h0 == pn_as_nat j n))) /\
+      exists (n:pn j nl). (wlog w h1 == Seq.snoc (wlog w h0) (Entry n ad p ne c) /\ wctrT w h0 == pn_as_nat j n))) /\
     modifies (Set.union (footprint w) (shared_footprint w)) h0 h1)
 
 //val adata_of_entry: #i:I.id -> stream_entry i -> GTot AEAD.adata
@@ -235,13 +261,13 @@ val decrypt
   (ensures fun h0 res h1 ->
     rinvariant r h1 /\
     modifies (Set.union (rfootprint r) (rshared_footprint r)) h0 h1 /\
-    (None? res ==> read_pnT r h1 == read_pnT r h0) /\
+    (None? res ==> pnlogT r h1 == pnlogT r h0) /\
     (Flag.safeId i ==> (
       let lg = wlog w h0 in
       match (Seq.find_l (epn_filter i j ne) lg) with
         | None -> res = None
         | Some (Entry pn ad' #l' p _ c') ->
           if ad' = ad && l' = l && c' = c then
-            (res = Some p /\ read_pnT r h1 == Seq.snoc (read_pnT r h0) pn)
+            (res = Some p /\ pnlogT r h1 == Seq.snoc (pnlogT r h0) pn)
           else
             res = None)))
